Simple machine and Complex simulation

src/sequential/Simple.v
@@ -65,6 +65,12 @@ Definition is_acquire (e: ProgramEvent.t): bool :=
   | ProgramEvent.fence ordr ordw => Ordering.le Ordering.seqcst ordw || Ordering.le Ordering.acqrel ordr
   end.
 
+Definition is_syscall (e: ProgramEvent.t): bool :=
+  match e with
+  | ProgramEvent.syscall _ => true
+  | _ => false
+  end.
+
 
 Module Perm.
   Variant t: Type :=
@@ -288,6 +294,12 @@ Module Flag.
 
   Definition join (f0 f1: t): t := orb f0 f1.
 
+  Definition minus (f0 f1: t): t :=
+    match f1 with
+    | true => f0
+    | false => f1
+    end.
+
   Definition le (f0 f1: t): bool := implb f0 f1.
 
   Program Instance le_PreOrder: PreOrder le.
@@ -379,7 +391,9 @@ End Flag.
 Module Flags.
   Definition t := Loc.t -> Flag.t.
 
-  Definition empty: t := fun _ => false.
+  Definition top: t := fun _ => true.
+
+  Definition bot: t := fun _ => false.
 
   Definition is_empty (f: t): Prop := forall loc, f loc = false.
 
@@ -392,11 +406,20 @@ Module Flags.
   Definition sub (loc: Loc.t) (f: t): t :=
     fun loc' => if Loc.eq_dec loc' loc then false else (f loc').
 
+  Definition sub_opt (loc: option Loc.t) (f: t): t :=
+    match loc with
+    | Some loc => sub loc f
+    | None => f
+    end.
+
   Definition meet (f0 f1: t): t :=
     fun loc => Flag.meet (f0 loc) (f1 loc).
 
   Definition join (f0 f1: t): t :=
     fun loc => Flag.join (f0 loc) (f1 loc).
+
+  Definition minus (f0 f1: t): t :=
+    fun loc => Flag.minus (f0 loc) (f1 loc).
 
   Definition le (f0 f1: t): Prop :=
     forall loc, Flag.le (f0 loc) (f1 loc).
@@ -409,6 +432,18 @@ Module Flags.
   Next Obligation.
   Proof.
     ii. etrans; eauto.
+  Qed.
+
+  Lemma top_spec f:
+    le f top.
+  Proof.
+    ii. destruct f; ss.
+  Qed.
+
+  Lemma bot_spec f:
+    le bot f.
+  Proof.
+    ii. destruct f; ss.
   Qed.
 
   Lemma meet_le_l f0 f1:
@@ -498,9 +533,6 @@ Module ValueMap.
   Definition acquire (cond: Loc.t -> bool) (vs_acq: t) (vs: t): t :=
     fun loc => if (cond loc) then (vs loc) else (vs_acq loc).
 
-  Definition release (vs: t) (d: Flags.t): t :=
-    fun loc => if (d loc) then Const.undef else (vs loc).
-
   Definition le (vs0 vs1: t): Prop :=
     forall loc, Const.le (vs0 loc) (vs1 loc).
 
@@ -521,7 +553,6 @@ Module SeqMemory.
     mk {
         value_map: ValueMap.t;
         flags: Flags.t;
-        deferred: Flags.t;
       }.
 
   Definition read (loc: Loc.t) (m: t): Const.t :=
@@ -530,32 +561,31 @@ Module SeqMemory.
   Definition write (loc: Loc.t) (v: Const.t) (m: t): t :=
     mk (ValueMap.write loc v m.(value_map))
        (Flags.update loc true m.(flags))
-       (Flags.update loc false m.(deferred)).
+  .
 
   Variant acquire (cond: Loc.t -> bool) (v_acq: ValueMap.t):
     forall (m_before: t) (f: Flags.t) (m_after: t), Prop :=
   | acquire_intro
       m
-      (DEFERRED: Flags.is_empty m.(deferred))
     :
       acquire
         cond
         v_acq
         m
         (m.(flags))
-        (mk (ValueMap.acquire cond v_acq m.(value_map)) m.(flags) m.(deferred)).
+        (mk (ValueMap.acquire cond v_acq m.(value_map)) m.(flags))
+  .
 
   Variant release:
-    forall (m_before: t) (f_rel: Flags.t) (v_rel: ValueMap.t) (m_after: t), Prop :=
+    forall (m: t) (f_rel: Flags.t) (v_rel: ValueMap.t) (m_after: t), Prop :=
   | release_intro
-      d m
-      (DEFERRED: Flags.is_empty m.(deferred))
+      m
     :
       release
         m
-        (Flags.join d m.(flags))
-        (ValueMap.release m.(value_map) d)
-        (mk m.(value_map) Flags.empty d)
+        (m.(flags))
+        (m.(value_map))
+        (mk m.(value_map) Flags.bot)
   .
 
   Variant update:
@@ -566,7 +596,6 @@ Module SeqMemory.
       (m_after: t), Prop :=
   | update_intro
       m loc v_new
-      (DEFERRED: m.(deferred) loc = false)
     :
       update
         loc
@@ -575,18 +604,17 @@ Module SeqMemory.
         (m.(value_map) loc)
         (m.(flags) loc)
         (mk (ValueMap.write loc v_new m.(value_map))
-            (Flags.update loc false m.(flags))
-            (m.(deferred)))
+            (Flags.update loc false m.(flags)))
   .
 End SeqMemory.
 
 
-Module SeqEvent.
+Module Oracle.
   Record input :=
     mk_input {
         in_access: option (Loc.t * Const.t * Flag.t);
-        in_acquire: option (Flags.t);
-        in_release: option (ValueMap.t * Flags.t);
+        in_acquire: option (unit);
+        in_release: option (unit);
       }.
 
   Record output :=
@@ -595,59 +623,6 @@ Module SeqEvent.
         out_acquire: option (Perms.t * ValueMap.t);
         out_release: option (Perms.t);
       }.
-
-  Definition in_access_le (i0 i1: (Loc.t * Const.t * Flag.t)): Prop :=
-    match i0, i1 with
-    | (l0, v0, f0), (l1, v1, f1) =>
-      (<<LOC: l0 = l1>>) /\ (<<VAL: Const.le v0 v1>>) /\ (<<FLAG: Flag.le f0 f1>>)
-    end.
-
-  Definition in_acquire_le (i0 i1: Flags.t): Prop :=
-    (<<FLAG: Flags.le i0 i1>>).
-
-  Definition in_release_le (i0 i1: (ValueMap.t * Flags.t)): Prop :=
-    match i0, i1 with
-    | (v0, f0), (v1, f1) =>
-      (<<VAL: ValueMap.le v0 v1>>) /\ (<<FLAG: Flags.le f0 f1>>)
-    end.
-
-  Definition input_le (i0 i1: input): Prop :=
-    (<<ACCESS: option_rel in_access_le i0.(in_access) i1.(in_access)>>) /\
-    (<<ACQUIRE: option_rel in_acquire_le i0.(in_acquire) i1.(in_acquire)>>) /\
-    (<<RELEASE: option_rel in_release_le i0.(in_release) i1.(in_release)>>)
-  .
-
-  Program Instance in_access_le_PreOrder: PreOrder in_access_le.
-  Next Obligation.
-  Proof.
-    ii. unfold in_access_le. des_ifs. splits; refl.
-  Qed.
-  Next Obligation.
-  Proof.
-    ii. unfold in_access_le in *. des_ifs. des. splits; etrans; eauto.
-  Qed.
-
-  Program Instance in_acquire_le_PreOrder: PreOrder in_acquire_le.
-
-  Program Instance in_release_le_PreOrder: PreOrder in_release_le.
-  Next Obligation.
-  Proof.
-    ii. unfold in_release_le. des_ifs. splits; refl.
-  Qed.
-  Next Obligation.
-  Proof.
-    ii. unfold in_release_le in *. des_ifs. des. splits; etrans; eauto.
-  Qed.
-
-  Program Instance input_le_PreOrder: PreOrder input_le.
-  Next Obligation.
-  Proof.
-    ii. unfold input_le. splits; refl.
-  Qed.
-  Next Obligation.
-  Proof.
-    ii. unfold input_le in *. des. splits; etrans; eauto.
-  Qed.
 
   Definition wf_input (e: ProgramEvent.t) (i: input): Prop :=
     (<<UPDATE: forall loc,
@@ -662,14 +637,6 @@ Module SeqEvent.
     (<<RELEASE: is_some o.(out_release) <-> is_release e>>)
   .
 
-  Lemma wf_input_event_le e0 e1 i
-        (EVENT: ProgramEvent.le e0 e1)
-    :
-      wf_input e0 i <-> wf_input e1 i.
-  Proof.
-    unfold wf_input. destruct e0, e1; ss; des; clarify.
-  Qed.
-
   Lemma wf_output_event_le e0 e1 o
         (EVENT: ProgramEvent.le e0 e1)
     :
@@ -678,8 +645,148 @@ Module SeqEvent.
     unfold wf_output. destruct e0, e1; ss; des; clarify.
   Qed.
 
+  Record t :=
+    mk {
+        _t: Type;
+        _step: ProgramEvent.t -> input -> output -> _t -> _t -> Prop;
+        _o: _t;
+      }.
+
+  Variant step: forall (pe: ProgramEvent.t) (i: input) (o: output) (o0 o1: t), Prop :=
+  | step_intro
+      pe i o
+      _t (_step: ProgramEvent.t -> input -> output -> _t -> _t -> Prop)
+      (x0 x1: _t)
+      (STEP: _step pe i o x0 x1)
+    :
+      step pe i o (@mk _t _step x0) (@mk _t _step x1)
+  .
+
+  Definition progress pe o0: Prop :=
+    forall i (WF: wf_input pe i),
+    exists o o1, (<<STEP: step pe i o o0 o1>>) /\ (<<WF: wf_output pe o>>).
+
+  Variant _wf (wf: t -> Prop): t -> Prop :=
+  | wf_intro
+      (o0: t)
+      (WF: forall pe i o o1 (STEP: step pe i o o0 o1),
+          (<<INPUT: wf_input pe i>>) /\
+          (<<OUTPUT: wf_output pe o>>) /\
+          (<<ORACLE: wf o1>>))
+      (LOAD: forall loc ord,
+          exists val, progress (ProgramEvent.read loc val ord) o0)
+      (STORE: forall loc ord val,
+          progress (ProgramEvent.write loc val ord) o0)
+      (FENCE: forall ordr ordw,
+          progress (ProgramEvent.fence ordr ordw) o0)
+    :
+      _wf wf o0
+  .
+
+  Lemma wf_mon: monotone1 _wf.
+  Proof.
+    ii. inv IN. econs; eauto. i.
+    exploit WF; eauto. i. des. splits; auto.
+  Qed.
+  #[export] Hint Resolve wf_mon: paco.
+
+  Definition wf := paco1 _wf bot1.
+End Oracle.
+
+
+Module SeqEvent.
+  Record input :=
+    mk_input {
+        in_access: option (Loc.t * Const.t * Flag.t);
+        in_acquire: option (Flags.t);
+        in_release: option (ValueMap.t * Flags.t);
+      }.
+
+  Definition written (i: input): Flags.t :=
+    Flags.join
+      (match i.(in_access) with
+       | Some (loc, _, true) => Flags.add loc Flags.bot
+       | _ => Flags.bot
+       end)
+      (match i.(in_release) with
+       | Some (_, f) => f
+       | _ => Flags.bot
+       end).
+
+  Definition deferred_step_wf
+             (i_src i_tgt: input)
+             (d0 d1: Flags.t): Prop :=
+    Flags.le (Flags.join d0 (written i_tgt)) (Flags.join d1 (written i_src)).
+
+  Definition get_oracle_input (i: input): Oracle.input :=
+    Oracle.mk_input
+      (i.(in_access))
+      (option_map (fun _ => tt) i.(in_acquire))
+      (option_map (fun _ => tt) i.(in_release))
+  .
+
+  Definition in_access_le (i0 i1: (Loc.t * Const.t * Flag.t)): Prop :=
+    match i0, i1 with
+    | (l0, v0, f0), (l1, v1, f1) =>
+      (<<LOC: l0 = l1>>) /\ (<<VAL: Const.le v0 v1>>) /\
+      (<<FLAG: Flag.le f0 f1>>)
+    end.
+
+  Definition in_acquire_le (i0 i1: Flags.t): Prop :=
+    (<<FLAG: Flags.le i0 i1>>).
+
+  Definition in_release_le (i0 i1: (ValueMap.t * Flags.t)): Prop :=
+    match i0, i1 with
+    | (v0, f0), (v1, f1) =>
+      (<<VAL: ValueMap.le v0 v1>>) /\
+      (<<FLAG: Flags.le f0 f1>>)
+    end.
+
+  Definition input_le (i0 i1: input): Prop :=
+    (<<ACCESS: option_rel in_access_le i0.(in_access) i1.(in_access)>>) /\
+    (<<ACQUIRE: option_rel in_acquire_le i0.(in_acquire) i1.(in_acquire)>>) /\
+    (<<RELEASE: option_rel in_release_le i0.(in_release) i1.(in_release)>>)
+  .
+
+  Definition in_access_match (d: Flags.t) (i_src i_tgt: (Loc.t * Const.t * Flag.t)): Prop :=
+    match i_tgt, i_src with
+    | (l0, v0, f0), (l1, v1, f1) =>
+      (<<LOC: l0 = l1>>) /\ (<<VAL: Const.le v0 v1>>) /\
+      (<<FLAG: Flag.le (Flag.join f0 (d l0)) f1>>)
+    end.
+
+  Definition in_acquire_match (d: Flags.t) (i_src i_tgt: Flags.t): Prop :=
+    (<<FLAG: Flags.le (Flags.join d i_tgt) i_src>>).
+
+  Definition in_release_match (d: Flags.t) (i_src i_tgt: (ValueMap.t * Flags.t)): Prop :=
+    match i_tgt, i_src with
+    | (v0, f0), (v1, f1) =>
+      (<<VAL: forall loc (UNDEFERRED: d loc = false), Const.le (v0 loc) (v1 loc)>>)
+    end.
+
+  Definition input_match (d: Flags.t) (i0 i1: input): Prop :=
+    (<<ACCESS: option_rel (in_access_match d) i0.(in_access) i1.(in_access)>>) /\
+    (<<ACQUIRE: option_rel (in_acquire_match d) i0.(in_acquire) i1.(in_acquire)>>) /\
+    (<<RELEASE: option_rel (in_release_match d) i0.(in_release) i1.(in_release)>>)
+  .
+
+  Definition wf_input (e: ProgramEvent.t) (i: input): Prop :=
+    (<<UPDATE: forall loc,
+        ((exists v_old f_old, i.(in_access) = Some (loc, v_old, f_old)) <-> is_accessing e = Some loc)>>) /\
+    (<<ACQUIRE: is_some i.(in_acquire) <-> is_acquire e>>) /\
+    (<<RELEASE: is_some i.(in_release) <-> is_release e>>)
+  .
+
+  Lemma wf_input_event_le e0 e1 i
+        (EVENT: ProgramEvent.le e0 e1)
+    :
+      wf_input e0 i <-> wf_input e1 i.
+  Proof.
+    unfold wf_input. destruct e0, e1; ss; des; clarify.
+  Qed.
+
   Variant step_update:
-    forall (i: option (Loc.t * Const.t * Flag.t))(o: option (Perm.t * Const.t))
+    forall (i: option (Loc.t * Const.t * Flag.t)) (o: option (Perm.t * Const.t))
            (p0: Perms.t) (m0: SeqMemory.t) (p1: Perms.t) (m1: SeqMemory.t), Prop :=
   | step_update_none
       p m
@@ -739,13 +846,13 @@ Module SeqEvent.
   .
 
   Variant step:
-    forall (i: input) (o: output)
+    forall (i: input) (o: Oracle.output)
            (p0: Perms.t) (m0: SeqMemory.t) (p1: Perms.t) (m1: SeqMemory.t), Prop :=
   | step_intro
       i o p0 m0 p1 m1 p2 m2 p3 m3
-      (UPD: step_update i.(in_access) o.(out_access) p0 m0 p1 m1)
-      (ACQ: step_acquire i.(in_acquire) o.(out_acquire) p1 m1 p2 m2)
-      (REL: step_release i.(in_release) o.(out_release) p2 m2 p3 m3)
+      (UPD: step_update i.(in_access) o.(Oracle.out_access) p0 m0 p1 m1)
+      (ACQ: step_acquire i.(in_acquire) o.(Oracle.out_acquire) p1 m1 p2 m2)
+      (REL: step_release i.(in_release) o.(Oracle.out_release) p2 m2 p3 m3)
     :
       step i o p0 m0 p3 m3
   .
@@ -837,55 +944,6 @@ End LANG.
 End SeqState.
 
 
-Module Oracle.
-  Record t :=
-    mk {
-        _t: Type;
-        _step: ProgramEvent.t -> SeqEvent.input -> SeqEvent.output -> _t -> _t -> Prop;
-        _o: _t;
-      }.
-
-  Variant step: forall (pe: ProgramEvent.t) (i: SeqEvent.input) (o: SeqEvent.output) (o0 o1: t), Prop :=
-  | step_intro
-      pe i o
-      _t (_step: ProgramEvent.t -> SeqEvent.input -> SeqEvent.output -> _t -> _t -> Prop)
-      (x0 x1: _t)
-      (STEP: _step pe i o x0 x1)
-    :
-      step pe i o (@mk _t _step x0) (@mk _t _step x1)
-  .
-
-  Definition progress pe o0: Prop :=
-    forall i (WF: SeqEvent.wf_input pe i),
-    exists o o1, (<<STEP: step pe i o o0 o1>>) /\ (<<WF: SeqEvent.wf_output pe o>>).
-
-  Variant _wf (wf: t -> Prop): t -> Prop :=
-  | wf_intro
-      (o0: t)
-      (WF: forall pe i o o1 (STEP: step pe i o o0 o1),
-          (<<INPUT: SeqEvent.wf_input pe i>>) /\
-          (<<OUTPUT: SeqEvent.wf_output pe o>>) /\
-          (<<ORACLE: wf o1>>))
-      (LOAD: forall loc ord,
-          exists val, progress (ProgramEvent.read loc val ord) o0)
-      (STORE: forall loc ord val,
-          progress (ProgramEvent.write loc val ord) o0)
-      (FENCE: forall ordr ordw,
-          progress (ProgramEvent.fence ordr ordw) o0)
-    :
-      _wf wf o0
-  .
-
-  Lemma wf_mon: monotone1 _wf.
-  Proof.
-    ii. inv IN. econs; eauto. i.
-    exploit WF; eauto. i. des. splits; auto.
-  Qed.
-  #[export] Hint Resolve wf_mon: paco.
-
-  Definition wf := paco1 _wf bot1.
-End Oracle.
-
 
 Module SeqThread.
 Section LANG.
@@ -918,7 +976,7 @@ Section LANG.
   Qed.
 
   Variant at_step:
-    forall (e: ProgramEvent.t) (i: SeqEvent.input) (o: SeqEvent.output)
+    forall (e: ProgramEvent.t) (i: SeqEvent.input) (o: Oracle.output)
            (th0: t) (th1: t), Prop :=
   | at_step_intro
       e0 e1 i0 i1 o
@@ -926,7 +984,7 @@ Section LANG.
       (LANG: lang.(Language.step) e1 st0 st1)
       (EVENT: ProgramEvent.le e0 e1)
       (INPUT: SeqEvent.input_le i0 i1)
-      (ORACLE: Oracle.step e0 i0 o o0 o1)
+      (ORACLE: Oracle.step e0 (SeqEvent.get_oracle_input i0) o o0 o1)
       (MEM: SeqEvent.step i1 o p0 m0 p1 m1)
     :
       at_step e0 i0 o (mk (SeqState.mk _ st0 m0) p0 o0) (mk (SeqState.mk _ st1 m1) p1 o1)
@@ -944,14 +1002,32 @@ Section LANG.
   Definition failure (th0: t): Prop :=
     exists th1, (<<FAILURE: step MachineEvent.failure th0 th1>>).
 
-  Variant non_acquire_step (e: MachineEvent.t) (th0: t) (th1: t): Prop :=
-  | non_acquire_step_na_step
-      (STEP: na_step e th0 th1)
-  | non_acquire_step_at_step
-      pe i o
-      (ACQUIRE: ~ is_acquire pe)
-      (EVENT: e = get_machine_event pe)
+  Inductive non_acquire_steps: forall (d: Flags.t) (th0: t) (th1: t), Prop :=
+  | non_acquire_steps_base
+      th
+    :
+      non_acquire_steps th.(state).(SeqState.memory).(SeqMemory.flags) th th
+  | non_acquire_steps_failure
+      th
+      (FAIL: failure th)
+    :
+      non_acquire_steps Flags.top th th
+  | non_acquire_steps_na_step
+      th0 th1 th2 d
+      (STEP: na_step MachineEvent.silent th0 th1)
+      (STEPS: non_acquire_steps d th1 th2)
+    :
+      non_acquire_steps d th0 th2
+  | non_acquire_steps_at_step
+      th0 th1 th2 pe i o d
       (STEP: at_step pe i o th0 th1)
+      (STEPS: non_acquire_steps d th1 th2)
+      (ACQUIRE: ~ is_acquire pe)
+      (SILENT: get_machine_event pe = MachineEvent.silent)
+    :
+      non_acquire_steps
+        (Flags.join (SeqEvent.written i) (Flags.sub_opt (is_accessing pe) d))
+        th0 th2
   .
 End LANG.
 End SeqThread.
@@ -964,42 +1040,41 @@ Section SIMULATION.
   Variable sim_terminal: forall (st_src:(Language.state lang_src)) (st_tgt:(Language.state lang_tgt)), Prop.
 
   Definition sim_seq_terminal_case
-             (p0: Perms.t)
+             (p0: Perms.t) (d0: Flags.t)
              (st_src0: SeqState.t lang_src)
              (st_tgt0: SeqState.t lang_tgt): Prop :=
-    forall (TERMINAL_TGT: lang_tgt.(Language.is_terminal) st_tgt0.(SeqState.state))
-           (DEFERRED: Flags.is_empty st_tgt0.(SeqState.memory).(SeqMemory.deferred)),
+    forall (TERMINAL_TGT: lang_tgt.(Language.is_terminal) st_tgt0.(SeqState.state)),
     exists st_src1,
       (<<STEPS: rtc (SeqState.na_step p0 MachineEvent.silent) st_src0 st_src1>>) /\
       (<<TERMINAL_SRC: lang_src.(Language.is_terminal) st_src1.(SeqState.state)>>) /\
       (<<TERMINAL: sim_terminal st_src1.(SeqState.state) st_tgt0.(SeqState.state)>>) /\
       (<<VALUE: ValueMap.le st_tgt0.(SeqState.memory).(SeqMemory.value_map) st_tgt0.(SeqState.memory).(SeqMemory.value_map)>>) /\
-      (<<FLAG: Flags.le st_tgt0.(SeqState.memory).(SeqMemory.flags) st_tgt0.(SeqState.memory).(SeqMemory.flags)>>) /\
-      (<<DEFERRED: Flags.is_empty st_src0.(SeqState.memory).(SeqMemory.deferred)>>)
+      (<<FLAG: Flags.le st_tgt0.(SeqState.memory).(SeqMemory.flags) (Flags.join d0 st_tgt0.(SeqState.memory).(SeqMemory.flags))>>)
   .
 
   Definition sim_seq_na_step_case
              (sim_seq:
                 forall
-                  (p0: Perms.t)
+                  (p0: Perms.t) (d0: Flags.t)
                   (st_src0: SeqState.t lang_src)
                   (st_tgt0: SeqState.t lang_tgt), Prop)
-             (p0: Perms.t)
+             (p0: Perms.t) (d0: Flags.t)
              (st_src0: SeqState.t lang_src)
              (st_tgt0: SeqState.t lang_tgt): Prop :=
     forall st_tgt1 e (STEP_TGT: SeqState.na_step p0 e st_tgt0 st_tgt1),
     exists st_src1 st_src2,
       (<<STEPS: rtc (SeqState.na_step p0 MachineEvent.silent) st_src0 st_src1>>) /\
       (<<STEP: SeqState.na_opt_step p0 e st_src1 st_src2>>) /\
-      (<<SIM: sim_seq p0 st_src2 st_tgt1>>).
+      (<<SIM: sim_seq p0 d0 st_src2 st_tgt1>>)
+  .
 
   Definition sim_seq_at_step_case
              (sim_seq:
                 forall
-                  (p0: Perms.t)
+                  (p0: Perms.t) (d0: Flags.t)
                   (st_src0: SeqState.t lang_src)
                   (st_tgt0: SeqState.t lang_tgt), Prop)
-             (p0: Perms.t)
+             (p0: Perms.t) (d0: Flags.t)
              (st_src0: SeqState.t lang_src)
              (st_tgt0: SeqState.t lang_tgt): Prop :=
     forall st_tgt1 e_tgt
@@ -1011,58 +1086,61 @@ Section SIMULATION.
       (<<EVENT: ProgramEvent.le e_src e_tgt>>) /\
       (<<SIM: forall i_tgt o p1 mem_tgt
                      (INPUT: SeqEvent.wf_input e_tgt i_tgt)
-                     (OUTPUT: SeqEvent.wf_output e_tgt o)
+                     (OUTPUT: Oracle.wf_output e_tgt o)
                      (STEP_TGT: SeqEvent.step i_tgt o p0 st_tgt0.(SeqState.memory) p1 mem_tgt),
-          exists i_src mem_src,
+          exists i_src mem_src d1,
             (<<STEP_SRC: SeqEvent.step i_src o p0 st_src1.(SeqState.memory) p1 mem_src>>) /\
-            (<<INPUT: SeqEvent.input_le i_tgt i_src>>) /\
+            (<<DEFERRED: SeqEvent.deferred_step_wf i_src i_tgt d0 d1>>) /\
+            (<<MATCH: SeqEvent.input_match d1 i_src i_tgt>>) /\
             (<<SIM: sim_seq p1
+                            d1
                             (SeqState.mk _ st_src2 mem_src)
-                            (SeqState.mk _ st_tgt1 mem_tgt)>>)>>).
+                            (SeqState.mk _ st_tgt1 mem_tgt)>>)>>)
+  .
 
   Definition sim_seq_partial_case
-             (p0: Perms.t)
+             (p0: Perms.t) (d0: Flags.t)
              (st_src0: SeqState.t lang_src)
              (st_tgt0: SeqState.t lang_tgt): Prop :=
-    forall o (WF: Oracle.wf o)
-           (DEFERRED: Flags.is_empty st_tgt0.(SeqState.memory).(SeqMemory.deferred)),
-    exists th,
-      (<<STEPS: rtc (SeqThread.non_acquire_step MachineEvent.silent) (SeqThread.mk st_src0 p0 o) th>>) /\
-      ((<<FLAG: Flags.le st_tgt0.(SeqState.memory).(SeqMemory.flags) th.(SeqThread.state).(SeqState.memory).(SeqMemory.flags)>>) /\
-       (<<DEFERRED: Flags.is_empty th.(SeqThread.state).(SeqState.memory).(SeqMemory.deferred)>>)
-       \/ (<<FAILURE: SeqThread.failure th>>)).
+    forall o (WF: Oracle.wf o),
+    exists th w,
+      (<<STEPS: SeqThread.non_acquire_steps w (SeqThread.mk st_src0 p0 o) th>>) /\
+      (<<FLAGS: Flags.le (Flags.join d0 st_tgt0.(SeqState.memory).(SeqMemory.flags)) w>>)
+  .
 
   Definition sim_seq_failure_case
-             (p0: Perms.t)
+             (p0: Perms.t) (d0: Flags.t)
              (st_src0: SeqState.t lang_src): Prop :=
     forall o (WF: Oracle.wf o),
-    exists th,
-      (<<STEPS: rtc (SeqThread.non_acquire_step MachineEvent.silent) (SeqThread.mk st_src0 p0 o) th>>) /\
-      (<<FAILURE: SeqThread.failure th>>).
+    exists th w,
+      (<<STEPS: SeqThread.non_acquire_steps w (SeqThread.mk st_src0 p0 o) th>>) /\
+      (<<FLAGS: Flags.le d0 w>>) /\
+      (<<FAILURE: SeqThread.failure th>>)
+  .
 
 
   Variant _sim_seq
           (sim_seq:
              forall
-               (p0: Perms.t)
+               (p0: Perms.t) (d0: Flags.t)
                (st_src0: SeqState.t lang_src)
                (st_tgt0: SeqState.t lang_tgt), Prop)
-          (p0: Perms.t)
+          (p0: Perms.t) (d0: Flags.t)
           (st_src0: SeqState.t lang_src)
           (st_tgt0: SeqState.t lang_tgt): Prop :=
   | sim_seq_normal
-      (TERMINAL: sim_seq_terminal_case p0 st_src0 st_tgt0)
-      (NASTEP: sim_seq_na_step_case sim_seq p0 st_src0 st_tgt0)
-      (ATSTEP: sim_seq_at_step_case sim_seq p0 st_src0 st_tgt0)
-      (PARTIAL: sim_seq_partial_case p0 st_src0 st_tgt0)
+      (TERMINAL: sim_seq_terminal_case p0 d0 st_src0 st_tgt0)
+      (NASTEP: sim_seq_na_step_case sim_seq p0 d0 st_src0 st_tgt0)
+      (ATSTEP: sim_seq_at_step_case sim_seq p0 d0 st_src0 st_tgt0)
+      (PARTIAL: sim_seq_partial_case p0 d0 st_src0 st_tgt0)
   | sim_seq_failure
-      (FAILURE: sim_seq_failure_case p0 st_src0)
+      (FAILURE: sim_seq_failure_case p0 d0 st_src0)
   .
 
-  Definition sim_seq := paco3 _sim_seq bot3.
+  Definition sim_seq := paco4 _sim_seq bot4.
   Arguments sim_seq: clear implicits.
 
-  Lemma sim_seq_mon: monotone3 _sim_seq.
+  Lemma sim_seq_mon: monotone4 _sim_seq.
   Proof.
     ii. inv IN.
     { econs 1; eauto.
@@ -1074,28 +1152,29 @@ Section SIMULATION.
   Qed.
 
 
-  Lemma sim_seq_partial_imm p st_src st_tgt
-        (FLAGS: Flags.le st_tgt.(SeqState.memory).(SeqMemory.flags) st_src.(SeqState.memory).(SeqMemory.flags))
-        (DEFERRED: Flags.is_empty st_tgt.(SeqState.memory).(SeqMemory.deferred) -> Flags.is_empty st_src.(SeqState.memory).(SeqMemory.deferred))
+  Lemma sim_seq_partial_imm p d st_src st_tgt
+        (FLAGS: Flags.le (Flags.join d st_tgt.(SeqState.memory).(SeqMemory.flags)) st_src.(SeqState.memory).(SeqMemory.flags))
     :
-      sim_seq_partial_case p st_src st_tgt.
+      sim_seq_partial_case p d st_src st_tgt.
   Proof.
-    ii. esplits; [refl|]. left. splits; auto.
+    ii. esplits; [econs 1|]. ss.
   Qed.
 
-  Lemma sim_seq_failure_imm p0 st_src0 st_tgt0 st_src1
+  Lemma sim_seq_failure_imm p0 d st_src0 st_tgt0 st_src1
         (FAILURE: SeqState.na_step p0 MachineEvent.failure st_src0 st_src1)
     :
-      sim_seq p0 st_src0 st_tgt0.
+      sim_seq p0 d st_src0 st_tgt0.
   Proof.
-    pfold. right. red. i. esplits; [refl|].
-    econs. left. econs. eauto.
+    pfold. right. red. i. esplits.
+    { econs 2. econs. left. econs. eauto. }
+    { eapply Flags.top_spec. }
+    { econs. left. econs. eauto. }
   Qed.
 
   Definition sim_seq_all (st_src: lang_src.(Language.state)) (st_tgt: lang_tgt.(Language.state)): Prop :=
     forall p m,
       sim_seq
-        p
+        p Flags.bot
         (SeqState.mk _ st_src m)
         (SeqState.mk _ st_tgt m).
 End SIMULATION.
